Add a bunch more proof

src/examples/fast_exp.dfy
@@ -13,6 +13,43 @@ lemma exp_sum(b: nat, n1: nat, n2: nat)
   }
 }
 
+function bits(n: nat): seq<bool>
+  decreases n
+{
+  if n == 0 then []
+  else [if (n % 2 == 0) then false else true] + bits(n/2)
+}
+
+function from_bits(s: seq<bool>): nat {
+  if s == [] then 0
+  else (if s[0] then 1 else 0) + 2 * from_bits(s[1..])
+}
+
+lemma bits_from_bits(n: nat)
+  ensures from_bits(bits(n)) == n
+{
+}
+
+lemma bits_trim_front(n: nat)
+  requires n > 0
+  ensures from_bits(bits(n)[1..]) == n/2
+{}
+
+lemma from_bits_append(s: seq<bool>, b: bool)
+  ensures from_bits(s + [b]) == from_bits(s) + exp(2, |s|) * (if b then 1 else 0)
+{}
+
+lemma from_bits_sum(s1: seq<bool>, s2: seq<bool>)
+  ensures from_bits(s1 + s2) == from_bits(s1) + exp(2, |s1|) * from_bits(s2)
+{
+  if s2 == [] {
+  } else {
+    assert s2 == [s2[0]] + s2[1..];
+    from_bits_append(s1, s2[0]);
+    from_bits_sum(s1, s2[1..]);
+  }
+}
+
 method fast_exp(b: nat, n: nat) returns (r: nat)
   ensures r == exp(b, n)
 {
@@ -20,25 +57,40 @@ method fast_exp(b: nat, n: nat) returns (r: nat)
   var c := b;
   ghost var n0 := n;
   var n := n;
-  ghost var i := 0;
+  ghost var i: nat := 0;
+  bits_from_bits(n);
   while n > 0
     decreases n
     invariant c == exp(b, exp(2, i))
+    invariant n <= n0
+    invariant i <= |bits(n0)|
+    invariant bits(n) == bits(n0)[i..]
+    invariant n == from_bits(bits(n0)[i..])
+    invariant a == exp(b, from_bits(bits(n0)[..i]))
   {
+    ghost var n_loop_top := n;
     if n % 2 == 1 {
+      assert bits(n)[0] == true;
       // a accumulates sum(i => b^(2^n_i), i) where n_i are the 1 bits of n
-      // TODO: n-n0 is sum(i => 2^n_i, i), right?
+      // TODO: n0-n is sum(i => 2^n_i, i), right?
       a := a * c;
+      exp_sum(b, n0-n, i);
       // (n-1)/2 == n/2 in this case, but we want to be extra clear that we're
       // "dropping" a 1 bit here and so something interesting is happening
       n := (n-1) / 2;
+      assert 2 * exp(2, i) == exp(2, i+1);
+      assert a == exp(b, from_bits(bits(n0)[..i+1]));
     } else {
+      assert bits(n)[0] == false;
       n := n / 2;
+      assert a == exp(b, from_bits(bits(n0)[..i+1]));
     }
+    assert n == n_loop_top/2;
     c := c * c;
     exp_sum(b, exp(2, i), exp(2, i));
+    // assert bits(n0)[i+1..] == bits(n0)[i..][1..];
     i := i + 1;
   }
-  assert false;
+  assert bits(n0)[..i] == bits(n0);
   return a;
 }
